src/SimpleTypesNotations.v
@@ -1,8 +1,7 @@
 (** * Notations for Simple Types *)
+(*  This notation is in a separated file to avoid conflict with the Ltac in MyLtacs file *)
 
 Require Import SimpleTypes.
-
-Unset Printing Notations.
 
 Declare Custom Entry DM.
 Notation "&[ e ]" := e (e custom DM at level 2).
@@ -14,5 +13,3 @@ Notation "( e )" := e (in custom DM, e at level 2).
 
 Notation "{ x }" := x (in custom DM, x constr).
 Notation "x" := x (in custom DM at level 0, x ident).
-
-Check forall tau, &[tau -> tau] = &[((tau -> tau) -> (tau))].
